src/cbor/raw/pulse/everparse/CBOR.Pulse.Raw.Test.fst
@@ -8,11 +8,12 @@ module SZ = FStar.SizeT
 
 ```pulse
 fn test (#pm: perm) (#v: Ghost.erased bytes) (s: slice byte)
-  requires pts_to s #pm v
+  requires pts_to s #pm v ** pure (exists off . validator_success test_parse 0sz v off)
   returns _: SZ.t
   ensures pts_to s #pm v
 {
 //  validate_nonempty (validate_and_read_elim validate_header) s 0sz
-  validate_nonempty (validate_and_read_elim validate_initial_byte) s 0sz
+//  validate_nonempty (validate_and_read_elim validate_initial_byte) s 0sz
+  test_jump s 0sz
 }
 ```
